verified-ocaml/instruct-verification/theories/CONST3_correct.v
@@ -22,7 +22,6 @@ Proof.
   intros e le m s. unfold handler_correct, handle_CONSTINT. simpl. intros ard Hpre _. unfold abs_rel_with_ard in Hpre. set (sb := ar_sptr_block ard) in *. set (so := ar_sptr_ofs ard) in *. set (hm := ar_heap_map ard) in *.
   destruct Hpre as (Hle_s & [pc_ptr [Hpc_load Hpc_rel]] & [accu_v [Haccu_load Haccu_repr]] & [sp_ptr [sp_b [sp_ofs [Hsp_load [Hsp_eq [Hstack_repr [Hsp_ne_sb [Hsp_ne_gb Hcb_ne_sp]]]]]]]] & [env_v [Henv_load Henv_repr]] & Hextra_load & [gd_ptr [Hgd_load [Hgd_eq [Hglobal_repr Hgb_ne_sb]]]] & [ts_ptr [Hts_load Htrap_rel]]). subst sp_ptr.
   pose proof (sptr_ofs_representable ard) as Hso_bound. fold so in Hso_bound. pose proof (Ptrofs.unsigned_range so) as [Hso_pos _].
-  pose proof (sp_block_ne_sptr ard sp_b) as Hblock_sep. fold sb in Hblock_sep. pose proof (global_block_ne_sptr ard) as Hgb_ne. fold sb in Hgb_ne.
   destruct interp_state_co as [co_is [Hco [Hsp_offset Haccu_offset]]].
   destruct (store_succeeds_from_load m sb (Ptrofs.unsigned so + 8) accu_v (Vlong (Int64.repr 7)) Haccu_load) as [m' Hstore].
   exists le. exists m'. exists (Out_return (Some (Vint (Int.repr 0), tint))). split.
@@ -41,10 +40,10 @@ Proof.
     { exact Hle_s. }
     { exists pc_ptr. split. exact Hpc_load'. simpl. exact Hpc_rel. }
     { exists (Vlong (Int64.repr 7)). split. exact Haccu_load'. simpl. exact (vr_int _ 3). }
-    { exists (Vptr sp_b sp_ofs), sp_b, sp_ofs. split; [| split; [| split; [| split; [| split]]]]. exact Hsp_load'. reflexivity. simpl. apply (stack_repr_store_other_block hm m m' _ sp_b sp_ofs sb (uso + 8) (Vlong (Int64.repr 7)) Hstack_repr Hstore). intro Heq; exact (Hblock_sep (eq_sym Heq)).
+    { exists (Vptr sp_b sp_ofs), sp_b, sp_ofs. split; [| split; [| split; [| split; [| split]]]]. exact Hsp_load'. reflexivity. simpl. apply (stack_repr_store_other_block hm m m' _ sp_b sp_ofs sb (uso + 8) (Vlong (Int64.repr 7)) Hstack_repr Hstore). intro Heq; exact (Hsp_ne_sb (eq_sym Heq)).
         exact Hsp_ne_sb. exact Hsp_ne_gb. exact Hcb_ne_sp. }
     { exists env_v. split. exact Henv_load'. simpl. exact Henv_repr. }
     { simpl. exact Hextra_load'. }
-    { exists gd_ptr. split; [| split; [| split]]. exact Hgd_load'. simpl. exact Hgd_eq. simpl. apply (global_repr_store_other_block hm m m' _ _ _ sb (uso + 8) (Vlong (Int64.repr 7)) Hglobal_repr Hstore). intro Heq2; exact (Hgb_ne (eq_sym Heq2)). exact Hgb_ne_sb. }
+    { exists gd_ptr. split; [| split; [| split]]. exact Hgd_load'. simpl. exact Hgd_eq. simpl. apply (global_repr_store_other_block hm m m' _ _ _ sb (uso + 8) (Vlong (Int64.repr 7)) Hglobal_repr Hstore). intro Heq2; exact (Hgb_ne_sb (eq_sym Heq2)). exact Hgb_ne_sb. }
     { exists ts_ptr. split. exact Hts_load'. simpl. exact Htrap_rel. } }
 Qed.
