verified-ocaml/instruct-verification/theories/GTINT_correct.v
@@ -109,7 +109,6 @@ Proof.
   destruct Hrange as [Ha_range Hb_range].
   pose proof (sptr_ofs_representable ard) as Hso_bound. fold so in Hso_bound.
   pose proof (Ptrofs.unsigned_range so) as [Hso_pos _].
-  pose proof (sp_block_ne_sptr ard sp_b) as Hblock_sep. fold sb in Hblock_sep.
   pose proof (global_block_ne_sptr ard) as Hgb_ne. fold sb in Hgb_ne.
   rewrite Haccu_eq in Haccu_repr. inversion Haccu_repr; subst accu_v. rename H0 into Haccu_is_int.
   rewrite Hstk in Hstack_repr.
@@ -123,7 +122,7 @@ Proof.
   assert (Haccu_load_m1 : Mem.load Mint64 m1 sb (Ptrofs.unsigned so + 8) = Some (Vlong (Int64.repr (a * 2 + 1)))).
   { apply (load_after_store_other m m1 sb (Ptrofs.unsigned so + 16) (Ptrofs.unsigned so + 8) new_sp_v (Vlong (Int64.repr (a * 2 + 1))) Hstore1 Haccu_load). left. lia. }
   assert (Hload_sp0_m1 : Mem.load Mint64 m1 sp_b (Ptrofs.unsigned sp_ofs) = Some (Vlong (Int64.repr (b * 2 + 1)))).
-  { erewrite Mem.load_store_other. exact Hload_sp0. exact Hstore1. left. exact Hblock_sep. }
+  { erewrite Mem.load_store_other. exact Hload_sp0. exact Hstore1. left. exact Hsp_ne_sb. }
   set (gt_bool := Int64.lt (Int64.repr (b * 2 + 1)) (Int64.repr (a * 2 + 1))).
   set (result_v := Vlong (Int64.add (Int64.repr (if gt_bool then 2 else 0)) (Int64.repr 1))).
   destruct (store_succeeds_from_load m1 sb (Ptrofs.unsigned so + 8) (Vlong (Int64.repr (a * 2 + 1))) result_v Haccu_load_m1) as [m' Hstore2].
@@ -202,8 +201,8 @@ Proof.
       { simpl.
         eapply (stack_repr_store_other_block hm m1 m' _ sp_b (Ptrofs.add sp_ofs (Ptrofs.repr 8)) sb (uso + 8) result_v).
         + eapply (stack_repr_store_other_block hm m m1 _ sp_b (Ptrofs.add sp_ofs (Ptrofs.repr 8)) sb (uso + 16) new_sp_v).
-          * exact Hstack_repr_rest. * exact Hstore1. * intro Heq; exact (Hblock_sep (eq_sym Heq)).
-        + exact Hstore2. + intro Heq; exact (Hblock_sep (eq_sym Heq)). }
+          * exact Hstack_repr_rest. * exact Hstore1. * intro Heq; exact (Hsp_ne_sb (eq_sym Heq)).
+        + exact Hstore2. + intro Heq; exact (Hsp_ne_sb (eq_sym Heq)). }
       exact Hsp_ne_sb. exact Hsp_ne_gb. exact Hcb_ne_sp. }
     { exists env_v. split. exact Henv_load'. simpl. exact Henv_repr. }
     { simpl. exact Hextra_load'. }
