verified-ocaml/instruct-verification/theories/LSRINT_correct.v
@@ -244,7 +244,7 @@ Proof.
   change (Machine.stack s) with (Val_int b :: v_tl) in Hstep_pre.
   simpl in Hstep_pre. rename Hstep_pre into Hb.
   set (sb := ar_sptr_block ard) in *. set (so := ar_sptr_ofs ard) in *. set (hm := ar_heap_map ard) in *.
-  destruct Hpre as (Hle_s & [pc_ptr [Hpc_load Hpc_rel]] & [accu_v [Haccu_load Haccu_repr]] & [sp_ptr [sp_b [sp_ofs [Hsp_load [Hsp_eq [Hstack_repr [Hblock_sep [Hsp_ne_gb Hcb_ne_sp]]]]]]]] & [env_v [Henv_load Henv_repr]] & Hextra_load & [gd_ptr [Hgd_load [Hgd_eq [Hglobal_repr Hgb_ne]]]] & [ts_ptr [Hts_load Htrap_rel]]). subst sp_ptr.
+  destruct Hpre as (Hle_s & [pc_ptr [Hpc_load Hpc_rel]] & [accu_v [Haccu_load Haccu_repr]] & [sp_ptr [sp_b [sp_ofs [Hsp_load [Hsp_eq [Hstack_repr [Hsp_ne_sb [Hsp_ne_gb Hcb_ne_sp]]]]]]]] & [env_v [Henv_load Henv_repr]] & Hextra_load & [gd_ptr [Hgd_load [Hgd_eq [Hglobal_repr Hgb_ne]]]] & [ts_ptr [Hts_load Htrap_rel]]). subst sp_ptr.
   pose proof (ar_sptr_ofs_bound ard) as Hso_bound. fold so in Hso_bound.
   pose proof (Ptrofs.unsigned_range so) as [Hso_pos _].
   rewrite Haccu_eq in Haccu_repr. inversion Haccu_repr; subst accu_v. rename H0 into Haccu_is_int.
@@ -259,7 +259,7 @@ Proof.
   assert (Haccu_load_m1 : Mem.load Mint64 m1 sb (Ptrofs.unsigned so + 8) = Some (Vlong (Int64.repr (a * 2 + 1)))).
   { apply (load_after_store_other m m1 sb (Ptrofs.unsigned so + 16) (Ptrofs.unsigned so + 8) new_sp_v (Vlong (Int64.repr (a * 2 + 1))) Hstore1 Haccu_load). left. lia. }
   assert (Hload_sp0_m1 : Mem.load Mint64 m1 sp_b (Ptrofs.unsigned sp_ofs) = Some (Vlong (Int64.repr (b * 2 + 1)))).
-  { erewrite Mem.load_store_other. exact Hload_sp0. exact Hstore1. left. exact Hblock_sep. }
+  { erewrite Mem.load_store_other. exact Hload_sp0. exact Hstore1. left. exact Hsp_ne_sb. }
   set (shift_amt := Int64.shr (Int64.repr (b * 2 + 1)) (Int64.repr 1)).
   pose proof (lsr_shift_amount_in_range b Hb) as Hltu.
   fold shift_amt in Hltu.
@@ -353,9 +353,9 @@ Proof.
       - exact Hsp_load'.
       - eapply (stack_repr_store_other_block hm m1 m' _ sp_b (Ptrofs.add sp_ofs (Ptrofs.repr 8)) sb (uso + 8) result_v).
         + eapply (stack_repr_store_other_block hm m m1 _ sp_b (Ptrofs.add sp_ofs (Ptrofs.repr 8)) sb (uso + 16) new_sp_v).
-          * exact Hstack_repr_rest. * exact Hstore1. * intro Heq; exact (Hblock_sep (eq_sym Heq)).
-        + exact Hstore2. + intro Heq; exact (Hblock_sep (eq_sym Heq)).
-      - exact Hblock_sep.
+          * exact Hstack_repr_rest. * exact Hstore1. * intro Heq; exact (Hsp_ne_sb (eq_sym Heq)).
+        + exact Hstore2. + intro Heq; exact (Hsp_ne_sb (eq_sym Heq)).
+      - exact Hsp_ne_sb.
       - exact Hsp_ne_gb.
       - exact Hcb_ne_sp. }
     { exists env_v. split. exact Henv_load'. simpl. exact Henv_repr. }
