verified-ocaml/instruct-verification/theories/MULINT_correct.v
@@ -154,7 +154,6 @@ Proof.
   destruct Hpre as (Hle_s & [pc_ptr [Hpc_load Hpc_rel]] & [accu_v [Haccu_load Haccu_repr]] & [sp_ptr [sp_b [sp_ofs [Hsp_load [Hsp_eq [Hstack_repr [Hsp_ne_sb [Hsp_ne_gb Hcb_ne_sp]]]]]]]] & [env_v [Henv_load Henv_repr]] & Hextra_load & [gd_ptr [Hgd_load [Hgd_eq [Hglobal_repr Hgb_ne_sb]]]] & [ts_ptr [Hts_load Htrap_rel]]). subst sp_ptr.
   pose proof (sptr_ofs_representable ard) as Hso_bound. fold so in Hso_bound.
   pose proof (Ptrofs.unsigned_range so) as [Hso_pos _].
-  pose proof (sp_block_ne_sptr ard sp_b) as Hblock_sep. fold sb in Hblock_sep.
   pose proof (global_block_ne_sptr ard) as Hgb_ne. fold sb in Hgb_ne.
   rewrite Haccu_eq in Haccu_repr. inversion Haccu_repr; subst accu_v. rename H0 into Haccu_is_int.
   rewrite Hstk in Hstack_repr.
@@ -168,7 +167,7 @@ Proof.
   assert (Haccu_load_m1 : Mem.load Mint64 m1 sb (Ptrofs.unsigned so + 8) = Some (Vlong (Int64.repr (a * 2 + 1)))).
   { apply (load_after_store_other m m1 sb (Ptrofs.unsigned so + 16) (Ptrofs.unsigned so + 8) new_sp_v (Vlong (Int64.repr (a * 2 + 1))) Hstore1 Haccu_load). left. lia. }
   assert (Hload_sp0_m1 : Mem.load Mint64 m1 sp_b (Ptrofs.unsigned sp_ofs) = Some (Vlong (Int64.repr (b * 2 + 1)))).
-  { erewrite Mem.load_store_other. exact Hload_sp0. exact Hstore1. left. exact Hblock_sep. }
+  { erewrite Mem.load_store_other. exact Hload_sp0. exact Hstore1. left. exact Hsp_ne_sb. }
   set (result_v := Vlong (Int64.add
     (Int64.shl
       (Int64.mul
@@ -249,8 +248,8 @@ Proof.
     { exists new_sp_v, sp_b, (Ptrofs.add sp_ofs (Ptrofs.repr 8)). split; [| split; [| split; [| split; [| split]]]]. exact Hsp_load'. reflexivity. simpl.
       eapply (stack_repr_store_other_block hm m1 m' _ sp_b (Ptrofs.add sp_ofs (Ptrofs.repr 8)) sb (uso + 8) result_v).
       + eapply (stack_repr_store_other_block hm m m1 _ sp_b (Ptrofs.add sp_ofs (Ptrofs.repr 8)) sb (uso + 16) new_sp_v).
-        * exact Hstack_repr_rest. * exact Hstore1. * intro Heq; exact (Hblock_sep (eq_sym Heq)).
-            + exact Hstore2. + intro Heq; exact (Hblock_sep (eq_sym Heq)).
+        * exact Hstack_repr_rest. * exact Hstore1. * intro Heq; exact (Hsp_ne_sb (eq_sym Heq)).
+            + exact Hstore2. + intro Heq; exact (Hsp_ne_sb (eq_sym Heq)).
       + exact Hsp_ne_sb. + exact Hsp_ne_gb. + exact Hcb_ne_sp. }
     { exists env_v. split. exact Henv_load'. simpl. exact Henv_repr. }
     { simpl. exact Hextra_load'. }
